# 111

\begin{aligned}
\hat{F}(x)\hat{G}(x)
&=\sum_{i\ge 0}a_i\frac{x^i}{i!}\sum_{j\ge 0}b_j\frac{x^j}{j!}\\
&=\sum_{n\ge 0}x^{n}\sum_{i=0}^na_ib_{n-i}\frac{1}{i!(n-i)!}\\
&=\sum_{n\ge 0}\frac{x^{n} }{n!}\sum_{i=0}^n\binom{n}{i}a_ib_{n-i}
\end{aligned}


\begin{cases}
x = b_{1}(\text{mod } a_{1}) \\
x = b_{2}(\text{mod } a_{2})\\
   \cdots \\
x = b_n (\text{mod } a_{n})
\end{cases}


$$
h(x) = f(x^p)
\\
h(x) = f^p(x)
\\
h(x) = \sum_{d|x}f(d)
\\
h(x) = f(x)g(x)
$$


$\mu(n)$ =
\begin{cases}
1&n = 1\\
0&n\text{含有平方因子}\\
(-1)^k&k\text{为}n\text{的本质不同质因子}
\end{cases}


\begin{aligned}
\left|\bigcup_{i=1}^k\overline{S_i}\right|
=&\sum_i\left|\overline{S_i}\right|
-\sum_{i,j}\left|\overline{S_i}\cap\overline{S_j}\right|
+\sum_{i,j,k}\left|\overline{S_i}\cap\overline{S_j}\cap\overline{S_k}\right|
-\cdots\\
&+(-1)^{k-1}\left|\bigcap_{i=1}^k\overline{S_i}\right|\\
=&\sum_i\binom{k+r-n_i-2}{k-1}
-\sum_{i,j}\binom{k+r-n_i-n_j-3}{k-1}+\sum_{i,j,k}\binom{k+r-n_i-n_j-n_k-4}{k-1}
-\cdots\\
&+(-1)^{k-1}\binom{k+r-\sum_{i=1}^kn_i-k-1}{k-1}
\end{aligned}


M = \begin{bmatrix}e(A_1,B_1)&e(A_1,B_2)&\cdots&e(A_1,B_n)\\
e(A_2,B_1)&e(A_2,B_2)&\cdots&e(A_2,B_n)\\
\vdots&\vdots&\ddots&\vdots\\
e(A_n,B_1)&e(A_n,B_2)&\cdots&e(A_n,B_n)\end{bmatrix}
